Work in progress

providers/evercrypt/EverCrypt.Hash.Incremental.fsti
@@ -19,97 +19,128 @@ module Hash = EverCrypt.Hash
 open FStar.HyperStack.ST
 open Spec.Hash.Definitions
 
-#reset-options "--max_fuel 0 --max_ifuel 0"
-
-module B = LowStar.Buffer
-module S = FStar.Seq
-module ST = FStar.HyperStack.ST
-module HS = FStar.HyperStack
-module G = FStar.Ghost
-
-module Hash = EverCrypt.Hash
-
-open FStar.HyperStack.ST
-open Spec.Hash.Definitions
-open FStar.Integers
-
-noeq
-type state a =
-| State:
-    hash_state: Hash.state a ->
-    buf: B.buffer UInt8.t { B.length buf = block_length a } ->
-    total_len: UInt64.t ->
-    state a
-
-let footprint #a (s: state a) h =
-  let State hash_state buf_ _ = s in
-  B.(loc_union (loc_addr_of_buffer buf_) (Hash.footprint hash_state h))
-
-let freeable #a (s: state a) h =
-  let State hash_state buf _ = s in
-  B.freeable buf /\ Hash.freeable h hash_state
-
-let preserves_freeable #a (s: state a) (h0 h1: HS.mem) =
-  let State hash_state buf _ = s in
-  Hash.preserves_freeable hash_state h0 h1
-
-#push-options "--max_ifuel 1"
-/// A lemma to be used by all clients, to show that a stateful operation that
-/// operates on a disjoint fragment of the heap preserves the invariants of this
-/// module. Note: it might be useful to call `Hash.fresh_is_disjoint` to turn
-/// the `fresh_loc` post-condition of create_in into a more useful
-/// `loc_disjoint` clause.
-let modifies_disjoint_preserves #a (l: B.loc) (h0 h1: HS.mem) (s: state a): Lemma
-  (requires (
-    let hash_state = State?.hash_state s in
-    B.modifies l h0 h1 /\
-    B.loc_disjoint l (footprint s h0) /\
-    Hash.invariant hash_state h0))
-  (ensures (
-    let hash_state = State?.hash_state s in
-    Hash.invariant hash_state h1 /\
-    Hash.repr hash_state h1 == Hash.repr hash_state h0 /\
-    footprint s h0 == footprint s h1))
-=
-  let hash_state = State?.hash_state s in
-  Hash.frame_invariant l hash_state h0 h1;
-  Hash.frame_invariant_implies_footprint_preservation l hash_state h0 h1
-#pop-options
-
-noextract
-let split_at_last (a: Hash.alg) (b: bytes):
-  Pure (bytes_blocks a & bytes)
-    (requires True)
-    (ensures (fun (blocks, rest) ->
-      S.length rest < block_length a /\
-      S.length rest = S.length b % block_length a /\
-      S.equal (S.append blocks rest) b /\
-      S.length blocks % block_length a = 0))
-=
-  let n = S.length b / block_length a in
-  let blocks, rest = S.split b (n * block_length a) in
-  assert (S.length blocks = n * block_length a);
-  assert ((n * block_length a) % block_length a = 0);
-  assert (S.length rest = S.length b - n * block_length a);
-  assert (S.length b - n * block_length a < block_length a);
-  blocks, rest
-
 #set-options "--max_fuel 0 --max_ifuel 0"
-unfold
-let hashes (#a: Hash.alg) (h: HS.mem) (s: state a) (b: bytes) =
-  let State hash_state buf_ total_len = s in
-  let blocks, rest = split_at_last a b in
-  S.length blocks + S.length rest = v total_len /\
-  S.length b = v total_len /\
-  v total_len < pow2 61 /\
-  B.live h buf_ /\
-  B.(loc_disjoint (loc_buffer buf_) (Hash.footprint hash_state h)) /\
-  Hash.invariant hash_state h /\
-  S.equal (Hash.repr hash_state h) (Spec.Hash.update_multi a (Spec.Hash.init a) blocks) /\
-  S.equal (S.slice (B.as_seq h buf_) 0 (v total_len % block_length a)) rest
+
+/// Convenience helpers, so that clients only ever need to refer to this module
+/// ---------------------------------------------------------------------------
+
+unfold noextract
+let alg = Hash.alg
+
+// TODO: replace with include {Spec,Hacl}.Hash.Definitions here
+
+/// Abstract footprints, with the same machinery as EverCrypt.Hash
+/// --------------------------------------------------------------
+///
+/// Differences from EverCrypt.Hash include: combined framing lemma, and order
+/// of arguments in line with ``B.as_seq``, etc. which take the memory
+/// first.
+
+[@CAbstractStruct]
+val state_s: alg -> Type0
+
+let state alg = B.pointer (state_s alg)
+
+val freeable (#a: alg) (h: HS.mem) (p: state a): Type0
+
+let preserves_freeable #a (s: state a) (h0 h1: HS.mem): Type0 =
+  freeable h0 s ==> freeable h1 s
+
+val footprint_s: #a:alg -> HS.mem -> state_s a -> GTot B.loc
+let footprint (#a:alg) (m: HS.mem) (s: state a) =
+  B.(loc_union (loc_addr_of_buffer s) (footprint_s m (B.deref m s)))
+
+unfold let loc_includes_union_l_footprint_s = EverCrypt.Hash.loc_includes_union_l_footprint_s
+unfold let loc_in = EverCrypt.Hash.loc_in
+unfold let loc_unused_in = EverCrypt.Hash.loc_unused_in
+unfold let fresh_loc = EverCrypt.Hash.fresh_loc
+unfold let fresh_is_disjoint = EverCrypt.Hash.fresh_is_disjoint
+
+val invariant_s: (#a:alg) -> HS.mem -> state_s a -> Type0
+let invariant (#a:alg) (m: HS.mem) (s: state a) =
+  B.live m s /\
+  B.(loc_disjoint (loc_addr_of_buffer s) (footprint_s m (B.deref m s))) /\
+  invariant_s m (B.get m s 0)
+
+val invariant_loc_in_footprint
+  (#a: alg)
+  (s: state a)
+  (m: HS.mem)
+: Lemma
+  (requires (invariant m s))
+  (ensures (loc_in (footprint m s) m))
+  [SMTPat (invariant m s)]
+
+/// Keeping track of the bytes hashed so far
+/// ----------------------------------------
+///
+/// We offer a stateful predicate that allows the client to tie a particular
+/// state to a sequence of bytes hashed so far.
 
 noextract
 let bytes = S.seq UInt8.t
+
+val hashes: #a:Hash.alg -> h:HS.mem -> s:state a -> b:bytes -> Type0
+
+val hash_fits: #a:Hash.alg -> h:HS.mem -> s:state a -> b:bytes -> Lemma
+  (requires hashes h s b)
+  (ensures (
+    S.length b < Spec.Hash.Definitions.max_input_length a))
+  [ SMTPat (hashes h s b) ]
+
+/// Central frame invariants
+/// ------------------------
+///
+/// Everything a client needs to know when they modify something **disjoint**
+/// from a hash state.
+///
+/// Note that the distinction between invariant and hashes is kind of unclear --
+/// what should go in the invariant, what should be captured by the hashes
+/// predicate, since the two are so close to each other?
+///
+/// Perhaps it would've been easier to have an erased field in the internal
+/// state to keep track of the bytes hashed so far, which would've allowed a
+/// function ``val hashed: HS.mem -> state -> bytes`` instead of adding an extra
+/// framing lemma.
+///
+/// Note that the three framing lemmas are most general. We could bundle
+/// invariant and freeable (hence committing to always heap-allocating); we
+/// could also bundle invariant and hashes (hence preventing clients from
+/// performing any operations in-between their call to ``create_in`` and
+/// ``init`` since only one of the two pre-conditions would be established).
+///
+/// Note: it might be useful to call `Hash.fresh_is_disjoint` to turn the
+/// `fresh_loc` post-condition of create_in into a more useful `loc_disjoint`
+/// clause.
+
+
+val frame_invariant: #a:alg -> l:B.loc -> s:state a -> h0:HS.mem -> h1:HS.mem -> Lemma
+  (requires (
+    invariant h0 s /\
+    B.loc_disjoint l (footprint h0 s) /\
+    B.modifies l h0 h1))
+  (ensures (
+    invariant h1 s /\
+    footprint h0 s == footprint h1 s))
+
+val frame_hashes: #a:alg -> l:B.loc -> s:state a -> b:bytes -> h0:HS.mem -> h1:HS.mem -> Lemma
+  (requires (
+    invariant h0 s /\
+    hashes h0 s b /\
+    B.loc_disjoint l (footprint h0 s) /\
+    B.modifies l h0 h1))
+  (ensures (hashes h1 s b))
+
+val frame_freeable: #a:alg -> l:B.loc -> s:state a -> h0:HS.mem -> h1:HS.mem -> Lemma
+  (requires (
+    invariant h0 s /\
+    freeable h0 s /\
+    B.loc_disjoint l (footprint h0 s) /\
+    B.modifies l h0 h1))
+  (ensures (freeable h1 s))
+
+/// Stateful API
+/// ------------
 
 (** @type: true
 *)
@@ -117,11 +148,22 @@ val create_in (a: Hash.alg) (r: HS.rid): ST (state a)
   (requires (fun _ ->
     HyperStack.ST.is_eternal_region r))
   (ensures (fun h0 s h1 ->
-    hashes h1 s S.empty /\
+    invariant h1 s /\
     B.(modifies loc_none h0 h1) /\
-    Hash.fresh_loc (footprint s h1) h0 h1 /\
-    B.(loc_includes (loc_region_only true r) (footprint s h1)) /\
-    freeable s h1))
+    fresh_loc (footprint h1 s) h0 h1 /\
+    B.(loc_includes (loc_region_only true r) (footprint h1 s)) /\
+    freeable h1 s))
+
+(** @type: true
+*)
+val init (a: Hash.alg) (s: state a): Stack unit
+  (requires (fun h0 ->
+    invariant h0 s))
+  (ensures (fun h0 _ h1 ->
+    preserves_freeable s h0 h1 /\
+    invariant h1 s /\
+    hashes h1 s S.empty /\
+    B.(modifies (footprint h0 s) h0 h1)))
 
 unfold
 let update_pre
@@ -132,11 +174,12 @@ let update_pre
   (len: UInt32.t)
   (h0: HS.mem)
 =
+  invariant h0 s /\
   hashes h0 s (G.reveal prev) /\
   B.live h0 data /\
-  v len = B.length data /\
-  S.length (G.reveal prev) + v len < pow2 61 /\
-  B.(loc_disjoint (loc_buffer data) (footprint s h0))
+  U32.v len = B.length data /\
+  S.length (G.reveal prev) + U32.v len < pow2 61 /\
+  B.(loc_disjoint (loc_buffer data) (footprint h0 s))
 
 unfold
 let update_post
@@ -147,12 +190,11 @@ let update_post
   (len: UInt32.t)
   (h0 h1: HS.mem)
 =
-  B.(modifies (footprint s h0) h0 h1) /\
-  footprint s h0 == footprint s' h1 /\
-  hashes h1 s' (Seq.append (G.reveal prev) (B.as_seq h0 data)) /\
   preserves_freeable s h0 h1 /\
-  State?.hash_state s == State?.hash_state s' /\
-  State?.buf s == State?.buf s'
+  invariant h1 s /\
+  B.(modifies (footprint h0 s) h0 h1) /\
+  footprint h0 s == footprint h1 s /\
+  hashes h1 s' (Seq.append (G.reveal prev) (B.as_seq h0 data))
 
 (** @type: true
 *)
@@ -175,15 +217,16 @@ let finish_st (a: Hash.alg) =
   dst: Hacl.Hash.Definitions.hash_t a ->
   Stack unit
     (requires fun h0 ->
+      invariant h0 s /\
       hashes h0 s (G.reveal prev) /\
       B.live h0 dst /\
-      B.(loc_disjoint (loc_buffer dst) (footprint s h0)))
+      B.(loc_disjoint (loc_buffer dst) (footprint h0 s)))
     (ensures fun h0 s' h1 ->
-      assert_norm (pow2 61 < pow2 125);
-      hashes h1 s (G.reveal prev) /\
       preserves_freeable s h0 h1 /\
-      footprint s h0 == footprint s h1 /\
-      B.(modifies (loc_union (loc_buffer dst) (footprint s h0)) h0 h1) /\
+      invariant h1 s /\
+      hashes h1 s (G.reveal prev) /\
+      footprint h0 s == footprint h1 s /\
+      B.(modifies (loc_union (loc_buffer dst) (footprint h0 s)) h0 h1) /\
       S.equal (B.as_seq h1 dst) (Spec.Hash.hash a (G.reveal prev)))
 
 (** @type: true
@@ -197,11 +240,7 @@ val free:
   s:state a ->
   ST unit
   (requires fun h0 ->
-    let State hash_state buf_ _ = s in
-    freeable s h0 /\
-    B.live h0 buf_ /\
-    B.(loc_disjoint (loc_buffer buf_) (Hash.footprint hash_state h0)) /\
-    Hash.invariant hash_state h0)
+    freeable h0 s /\
+    invariant h0 s)
   (ensures fun h0 _ h1 ->
-    B.modifies (footprint s h0) h0 h1)
-
+    B.modifies (footprint h0 s) h0 h1)
