providers/evercrypt/EverCrypt.Hash.fsti
@@ -116,7 +116,7 @@ let invariant (#a:alg) (s: state a) (m: HS.mem) =
 
 //18-07-06 as_acc a better name? not really a representation
 val repr: #a:alg ->
-  s:state a -> h:HS.mem { invariant s h } -> GTot (words_state a)
+  s:state a -> h:HS.mem -> GTot (words_state a)
 
 // Waiting for these to land in LowStar.Modifies
 let loc_in (l: M.loc) (h: HS.mem) =
